Step 1: disable the membership instance and fix all errors

src/Init/Data/Option/Instances.lean
@@ -19,12 +19,12 @@ theorem eq_of_eq_some {α : Type u} : ∀ {x y : Option α}, (∀z, x = some z �
 theorem eq_none_of_isNone {α : Type u} : ∀ {o : Option α}, o.isNone → o = none
   | none, _ => rfl
 
-instance : Membership α (Option α) := ⟨fun b a => b = some a⟩
+-- instance : Membership α (Option α) := ⟨fun b a => b = some a⟩
 
-@[simp] theorem mem_def {a : α} {b : Option α} : a ∈ b ↔ b = some a := .rfl
+-- @[simp] theorem mem_def {a : α} {b : Option α} : a ∈ b ↔ b = some a := .rfl
 
-instance [DecidableEq α] (j : α) (o : Option α) : Decidable (j ∈ o) :=
-  inferInstanceAs <| Decidable (o = some j)
+-- instance [DecidableEq α] (j : α) (o : Option α) : Decidable (j ∈ o) :=
+--   inferInstanceAs <| Decidable (o = some j)
 
 @[simp] theorem isNone_iff_eq_none {o : Option α} : o.isNone ↔ o = none :=
   ⟨Option.eq_none_of_isNone, fun e => e.symm ▸ rfl⟩
@@ -42,15 +42,15 @@ Try to use the Boolean comparisons `Option.isNone` or `Option.isSome` instead.
 @[inline] def decidable_eq_none {o : Option α} : Decidable (o = none) :=
   decidable_of_decidable_of_iff isNone_iff_eq_none
 
-instance {p : α → Prop} [DecidablePred p] : ∀ o : Option α, Decidable (∀ a, a ∈ o → p a)
-| none => isTrue nofun
-| some a =>
-  if h : p a then isTrue fun _ e => some_inj.1 e ▸ h
-  else isFalse <| mt (· _ rfl) h
+-- instance {p : α → Prop} [DecidablePred p] : ∀ o : Option α, Decidable (∀ a, a ∈ o → p a)
+-- | none => isTrue nofun
+-- | some a =>
+--   if h : p a then isTrue fun _ e => some_inj.1 e ▸ h
+--   else isFalse <| mt (· _ rfl) h
 
-instance {p : α → Prop} [DecidablePred p] : ∀ o : Option α, Decidable (Exists fun a => a ∈ o ∧ p a)
-| none => isFalse nofun
-| some a => if h : p a then isTrue ⟨_, rfl, h⟩ else isFalse fun ⟨_, ⟨rfl, hn⟩⟩ => h hn
+-- instance {p : α → Prop} [DecidablePred p] : ∀ o : Option α, Decidable (Exists fun a => a ∈ o ∧ p a)
+-- | none => isFalse nofun
+-- | some a => if h : p a then isTrue ⟨_, rfl, h⟩ else isFalse fun ⟨_, ⟨rfl, hn⟩⟩ => h hn
 
 /--
 Given an optional value and a function that can be applied when the value is `some`, returns the
@@ -80,7 +80,7 @@ none
 ```
 -/
 @[inline]
-def pbind : (o : Option α) → (f : (a : α) → a ∈ o → Option β) → Option β
+def pbind : (o : Option α) → (f : (a : α) → o = some a → Option β) → Option β
   | none, _ => none
   | some a, f => f a rfl
 
@@ -108,7 +108,7 @@ none
 -/
 @[inline] def pmap {p : α → Prop}
     (f : ∀ a : α, p a → β) :
-    (o : Option α) → (∀ a, a ∈ o → p a) → Option β
+    (o : Option α) → (∀ a, o = some a → p a) → Option β
   | none, _ => none
   | some a, H => f a (H a rfl)
 
@@ -139,7 +139,7 @@ some ⟨3, ⋯⟩
 none
 ```
 -/
-@[inline] def pelim (o : Option α) (b : β) (f : (a : α) → a ∈ o → β) : β :=
+@[inline] def pelim (o : Option α) (b : β) (f : (a : α) → o = some a → β) : β :=
   match o with
   | none => b
   | some a => f a rfl
@@ -176,13 +176,13 @@ Examples:
 instance : ForM m (Option α) α :=
   ⟨Option.forM⟩
 
-instance : ForIn' m (Option α) α inferInstance where
-  forIn' x init f := do
-    match x with
-    | none => return init
-    | some a =>
-      match ← f a rfl init with
-      | .done r | .yield r => return r
+-- instance : ForIn' m (Option α) α inferInstance where
+--   forIn' x init f := do
+--     match x with
+--     | none => return init
+--     | some a =>
+--       match ← f a rfl init with
+--       | .done r | .yield r => return r
 
 -- No separate `ForIn` instance is required because it can be derived from `ForIn'`.
 
